new MemLog: initial reps & simple procedures

src/MemLog.v
@@ -10,75 +10,218 @@ Require Import BasicProg.
 Require Import FunctionalExtensionality.
 Require Import Omega.
 Require Import Word.
+Require Import Rec.
+Require Import Array.
+Require Import Eqdep_dec.
 
 Import ListNotations.
 Set Implicit Arguments.
 
+Inductive logstate :=
+| NoTransaction (cur : mem)
+(* Don't touch the disk directly in this state. *)
+| ActiveTxn (old : mem) (cur : mem)
+(* A transaction is in progress.
+ * It started from the first memory and has evolved into the second.
+ * It has not committed yet. *)
+| FinishedTxn (cur : mem)
+(* A transaction has been finished and flushed to the log, but not committed yet. *)
+| CommittedTxn (cur : mem)
+(* A transaction has committed but the log has not been applied yet. *).
 
 Definition memstate := list LOG.logentry.
 
+Record xparams := {
+  (* The actual data region is everything that's not described here *)
+  LogHeader : addr; (* Store the header here *)
+  LogCommit : addr; (* Store true to apply after crash. *)
+
+  LogStart : addr; (* Start of log region on disk *)
+  LogLen : addr  (* Size of log region; length but still use addr type *)
+}.
+
+
 Module MEMLOG.
+
+  Definition header_type := Rec.RecF ([("length", Rec.WordF addrlen)]).
+  Definition header := Rec.data header_type.
+  Definition mk_header (len : nat) : header := ($ len, tt).
+
+  Theorem header_sz_ok : Rec.len header_type <= valulen.
+  Proof.
+    rewrite valulen_is. simpl. firstorder. (* this could be much faster, say with reflection *)
+  Qed.
+
+  Theorem plus_minus_header : Rec.len header_type + (valulen - Rec.len header_type) = valulen.
+  Proof.
+    apply le_plus_minus_r; apply header_sz_ok.
+  Qed.
+
+  Definition header_to_valu (h : header) : valu.
+    set (zext (Rec.to_word h) (valulen - Rec.len header_type)) as r.
+    rewrite plus_minus_header in r.
+    refine r.
+  Defined.
+
+  Definition valu_to_header (v : valu) : header.
+    apply Rec.of_word.
+    rewrite <- plus_minus_header in v.
+    refine (split1 _ _ v).
+  Defined.
+
+  Definition header_valu_id : forall h,
+    valu_to_header (header_to_valu h) = h.
+  Proof.
+    unfold valu_to_header, header_to_valu.
+    unfold eq_rec_r, eq_rec.
+    intros.
+    rewrite <- plus_minus_header.
+    do 2 rewrite <- eq_rect_eq_dec by (apply eq_nat_dec).
+    unfold zext.
+    rewrite split1_combine.
+    apply Rec.of_to_id.
+    simpl; destruct h; tauto.
+  Qed.
+
+  Definition addr_per_block := valulen / addrlen.
+  Definition descriptor_type := Rec.ArrayF (Rec.WordF addrlen) addr_per_block.
+  Definition descriptor := Rec.data descriptor_type.
+  Theorem descriptor_sz_ok : valulen = Rec.len descriptor_type.
+    simpl. unfold addr_per_block. rewrite valulen_is. reflexivity.
+  Qed.
+
+  Definition descriptor_to_valu (d : descriptor) : valu.
+    rewrite descriptor_sz_ok.
+    apply Rec.to_word; auto.
+  Defined.
+
+  Definition valu_to_descriptor (v : valu) : descriptor.
+    rewrite descriptor_sz_ok in v.
+    apply Rec.of_word; auto.
+  Defined.
+
+  Theorem valu_descriptor_id : forall v,
+    descriptor_to_valu (valu_to_descriptor v) = v.
+  Proof.
+    unfold descriptor_to_valu, valu_to_descriptor.
+    unfold eq_rec_r, eq_rec.
+    intros.
+    rewrite Rec.to_of_id.
+    rewrite <- descriptor_sz_ok.
+    do 2 rewrite <- eq_rect_eq_dec by (apply eq_nat_dec).
+    trivial.
+  Defined.
+
+  (** On-disk representation of the log *)
+  Definition log_rep xp m (ms : memstate) : pred :=
+     ((LogHeader xp) |-> header_to_valu (mk_header (length ms)) *
+      [[ LOG.valid_log m ms ]] *
+      (* For now, support just one descriptor block, at the start of the log. *)
+      [[ length ms <= wordToNat (LogLen xp) ]] *
+      [[ length ms <= addr_per_block ]] *
+      exists rest, (LogStart xp) |-> descriptor_to_valu (map fst ms ++ rest) *
+      array (LogStart xp ^+ $1) (map snd ms) $1 *
+      (* XXX use array for this too (with an exis)? *)
+      LOG.avail_region (LogStart xp ^+ $1 ^+ $ (length ms))
+                         (wordToNat (LogLen xp) - length ms))%pred.
+
+  Definition data_rep old : pred :=
+    diskIs old.
+
+  Definition cur_rep (old : mem) (ms : memstate) (cur : mem) : pred :=
+    [[ forall a, cur a = LOG.replay ms old a ]]%pred.
+
   Definition rep xp (st: logstate) (ms: memstate) :=
     match st with
+    | NoTransaction m =>
+      (LogCommit xp) |-> $0
+    * [[ ms = nil ]]
+    * data_rep m
+    * log_rep xp m nil
     | ActiveTxn old cur =>
-      exists curdisk, LOG.rep xp (ActiveTxn old curdisk)
-      * [[ forall a, cur a = LOG.replay ms curdisk a ]]
-      * [[ LOG.valid_log curdisk ms ]]
-    | _ => LOG.rep xp st * [[ ms = nil ]]
+      (LogCommit xp) |-> $0
+    * data_rep old (* Transactions are always completely buffered in memory. *)
+    * log_rep xp old nil
+    * cur_rep old ms cur
+    * [[ LOG.valid_log old ms ]]
+    | FinishedTxn cur =>
+      (LogCommit xp) |-> $0
+    * [[ ms = nil ]]
+    * exists old, data_rep old
+    * exists log, log_rep xp old log
+    * cur_rep old log cur
+    | CommittedTxn cur =>
+      (LogCommit xp) |-> $1
+    * [[ ms = nil ]]
+    * exists old, data_rep old
+    * exists log, log_rep xp old log
+    * cur_rep old log cur
     end%pred.
 
   Definition ms_empty := @nil LOG.logentry.
 
-  Definition init xp rx :=
-    LOG.init xp ;;
+  Definition init T xp rx : prog T :=
+    Write (LogHeader xp) (header_to_valu (mk_header 0)) ;;
+    Write (LogCommit xp) $0 ;;
     rx tt.
 
-  Hint Extern 0 (okToUnify (LOG.log_rep _ _ _) (LOG.log_rep _ _ _)) => constructor : okToUnify.
-  Hint Extern 0 (okToUnify (LOG.cur_rep _ _ _) (LOG.cur_rep _ _ _)) => constructor : okToUnify.
-  Hint Extern 0 (okToUnify (LOG.data_rep _) (LOG.data_rep _)) => constructor : okToUnify.
+  Hint Extern 0 (okToUnify (log_rep _ _ _) (log_rep _ _ _)) => constructor : okToUnify.
+  Hint Extern 0 (okToUnify (cur_rep _ _ _) (cur_rep _ _ _)) => constructor : okToUnify.
+  Hint Extern 0 (okToUnify (data_rep _) (data_rep _)) => constructor : okToUnify.
 
-  Theorem init_ok : forall xp rx rec,
-    {{ exists old F, F
-     * LOG.data_rep old
-     * LOG.avail_region (LogStart xp) (wordToNat (LogLen xp) * 2)
-     * (LogCommit xp) |->?
-     * (LogLength xp) |->?
-     * [[ {{ rep xp (NoTransaction old) ms_empty * F }} rx tt >> rec ]]
-     * [[ {{ any }} rec >> rec ]]
-    }} init xp rx >> rec.
+  Ltac log_unfold := unfold rep, data_rep, cur_rep, log_rep.
+
+  Theorem init_ok : forall xp,
+    {< old,
+    PRE    data_rep old *
+           LOG.avail_region (LogStart xp) (1 + wordToNat (LogLen xp)) *
+           (LogCommit xp) |->? *
+           (LogHeader xp) |->?
+    POST:r rep xp (NoTransaction old) ms_empty
+    CRASH  any
+    >} init xp.
   Proof.
-    unfold init, rep.
-    hoare.
+    unfold init; log_unfold.
+    intros.
+    hoare; try apply pimpl_any.
+
+    instantiate (a := valu_to_descriptor w1).
+    rewrite valu_descriptor_id.
+    cancel.
   Qed.
 
-  Definition begin xp rx :=
-    LOG.begin xp ;;
+  Definition begin T xp rx : prog T :=
+    Write (LogHeader xp) (header_to_valu (mk_header 0)) ;;
     rx ms_empty.
 
-  Theorem begin_ok: forall xp rx rec,
-    {{ exists m F, rep xp (NoTransaction m) ms_empty * F
-     * [[ forall ms', {{ rep xp (ActiveTxn m m) ms' * F }} rx ms' >> rec ]]
-     * [[ {{ rep xp (NoTransaction m) ms_empty * F }} rec >> rec ]]
-    }} begin xp rx >> rec.
+  Theorem begin_ok: forall xp,
+    {< m,
+    PRE    rep xp (NoTransaction m) ms_empty
+    POST:r rep xp (ActiveTxn m m) r
+    CRASH  rep xp (NoTransaction m) ms_empty \/ rep xp (ActiveTxn m m) ms_empty
+    >} begin xp.
   Proof.
-    unfold begin, rep.
+    unfold begin; log_unfold.
     hoare.
   Qed.
 
-  Definition abort xp (ms:memstate) rx :=
-    LOG.abort xp ;;
+  Definition abort T xp (ms:memstate) rx : prog T :=
+    Write (LogHeader xp) (header_to_valu (mk_header 0)) ;;
     rx tt.
 
-  Theorem abort_ok : forall xp ms rx rec,
-    {{ exists m1 m2 F, rep xp (ActiveTxn m1 m2) ms * F
-     * [[ {{ rep xp (NoTransaction m1) ms_empty * F }} rx tt >> rec ]]
-     * [[ {{ rep xp (NoTransaction m1) ms_empty * F
-          \/ rep xp (ActiveTxn m1 m2) ms * F }} rec >> rec ]]
-    }} abort xp ms rx >> rec.
+  Theorem abort_ok : forall xp ms,
+    {< m1 m2,
+    PRE    rep xp (ActiveTxn m1 m2) ms
+    POST:r rep xp (NoTransaction m1) ms_empty
+    CRASH  rep xp (ActiveTxn m1 m2) ms \/ rep xp (NoTransaction m1) ms_empty
+    >} abort xp ms.
   Proof.
-    unfold abort, rep.
+    unfold abort; log_unfold.
     hoare.
   Qed.
+
+
+
 
   Program Definition list_nil_dec (T: Type) (l: list T) : {l=nil} + {l<>nil} :=
     match l with
